Bit of progress on guess example

state/Examples.Guess.fst
@@ -18,7 +18,9 @@ type player_type a3p =
 
 type play_guess_type a3p =
   args:(player_type a3p & (int & (int & int))) ->
-  ST (resexn (bool & int)) (requires fun h0 -> inv a3p h0 /\ fst (snd (snd args)) < fst (snd args) /\ fst (snd args) < snd (snd (snd args))) (ensures fun h0 r h1 -> inv a3p h1 /\ h0 `hrel a3p` h1)
+  ST (resexn (bool & int)) 
+    (requires fun h0 -> inv a3p h0 /\ fst (snd (snd args)) < fst (snd args) /\ fst (snd args) < snd (snd (snd args))) 
+    (ensures fun h0 _ h1 -> inv a3p h1 /\ h0 `hrel a3p` h1)
 
 val play_guess : play_guess_type c3p
 let play_guess args =
@@ -50,25 +52,35 @@ let cb_spec (a3p:threep) : pck_spec =
     (fun _ -> post_poly_arrow a3p)
 
 let player_spec (a3p:threep) : pck_spec =
-  Spec10 false
-    ((int & int) & (guess: (mk_poly_arrow a3p int cmp)))
-    (witnessable_pair _ _ #(witnessable_pair _ _ #witnessable_int #witnessable_int) #(witnessable_arrow int cmp _ _))
+  (Spec10 false
+    ((int & int) & mk_poly_arrow a3p int cmp)
+    (poly_iface_is_exportable a3p ((int & int) & mk_poly_arrow a3p int cmp)).c_styp (** TODO: simplify here: (witnessable_pair _ _ #(witnessable_pair _ _ #witnessable_int #witnessable_int) #(witnessable_arrow int cmp _ _)) *)
     (fun x h0 -> inv a3p h0 /\ fst (fst x) < snd (fst x))
     int
     witnessable_int
-    (fun _ h0 _ h1 -> inv a3p h1 /\ hrel a3p h0 h1)
+    (fun _ h0 _ h1 -> inv a3p h1 /\ hrel a3p h0 h1))
+
+let player_hoc : hoc c3p (player_spec c3p) =
+  TrivialPost10 (fun _ -> ()) (fun _ _ -> ())
+
+// select_check c3p (argt1 s) unit
+//                         (pre_poly_arrow c3p #(argt1 s) #(wt_argt1 s))
+//                         (fun x _ _ h1 -> (pre1 s) x h1)
+// cb_check a3p (argt1 s) unit #c2 pre post x eh0
+// type cb_check a3p (t1:Type) (t2:Type) {| c2: witnessable t2 |}
+//   (pre:(t1 -> st_pre))
+//   (post:(x:t1 -> h0:heap -> st_post' t2 (pre x h0)))
+//   (x:t1)
+//   (eh0:FStar.Ghost.erased heap{pre x eh0}) =
+//   (r:t2 -> ST (resexn unit) (fun h1 -> post_poly_arrow a3p eh0 r h1) (fun h1 rck h1' ->
+//     h1 == h1' /\ (Inl? rck ==> post x eh0 r h1)))
+
 
 (** Stuck here: **)
 instance importable_player (a3p:threep) : safe_importable_to a3p (player_type a3p) (Node (player_spec a3p) Leaf Leaf) =
   safe_importable_arrow_safe10 
     a3p _ _
     #(poly_iface_is_exportable a3p _ #(poly_iface_pair a3p _ _ #(poly_iface_pair a3p int int) #(poly_iface_arrow a3p _ _ #(poly_iface_int a3p) #(poly_iface_cmp a3p))))
-    // #(exportable_pair a3p 
-    //   (int & int) 
-    //   (mk_poly_arrow a3p int cmp) 
-    //   _ _ 
-    //   #(exportable_pair a3p int int Leaf Leaf #(exportable_int a3p) #(exportable_int a3p))
-    //   #(exportable_arrow_no_err00 a3p int _ #(poly_iface_is_safely_importable a3p int) cmp _ #(poly_iface_is_exportable a3p cmp #(poly_iface_cmp a3p)) _ _))
     _ _ #(poly_iface_is_safely_importable a3p int #(poly_iface_int a3p))
     (fun x h0 -> inv a3p h0 /\ fst (fst x) < snd (fst x))
     (fun _ h0 _ h1 -> inv a3p h1 /\ hrel a3p h0 h1)
@@ -76,10 +88,49 @@ instance importable_player (a3p:threep) : safe_importable_to a3p (player_type a3
 instance args_importable a3p : importable_to a3p (player_type a3p & (int & (int & int))) _ =
   importable_pair a3p (player_type a3p) (int & (int & int)) _ Leaf #(safe_importable_is_importable a3p _ _ #(importable_player a3p))
 
-instance exportable_play_guess a3p : exportable_from a3p (play_guess_type a3p) _ =
+let play_guess_spec (a3p:threep) : pck_spec =
+  SpecErr10 true
+    (player_type a3p & (int & (int & int)))
+    (args_importable a3p).c_styp (** TODO: simply here with witnessable *)
+    (fun x h0 -> inv a3p h0 /\ fst (snd (snd x)) < fst (snd x) /\ fst (snd x) < snd (snd (snd x)))
+    (bool & int)
+    (exportable_pair a3p bool int Leaf Leaf).c_styp (** TODO: simply here with witnessable *)
+    (fun _ h0 _ h1 -> inv a3p h1 /\ hrel a3p h0 h1)
+
+let play_guess_hoc : hoc c3p (play_guess_spec c3p) =
+  EnforcePre10
+    (fun args ->
+      let args : (player_type c3p & (int & (int & int))) = args in
+      let eh0 = get_heap () in
+      let check : cb_check c3p (player_type c3p & (int & (int & int))) _ (pre_poly_arrow c3p #(argt1 (play_guess_spec c3p)) #(wt_argt1 (play_guess_spec c3p))) (fun x _ _ h1 -> (pre1 (play_guess_spec c3p)) x h1)  args eh0 =
+        (fun () -> if fst (snd (snd args)) < fst (snd args) && fst (snd args) < snd (snd (snd args)) then Inl () else Inr (Contract_failure "Invalid range")) in
+      (| eh0, check |))
+    (fun _ _ -> admit ())
+
+instance exportable_play_guess a3p : exportable_from a3p (play_guess_type a3p) (Node (play_guess_spec a3p) _ _) =
   exportable_arrow10 a3p 
     _ _ _ _ 
     #(args_importable a3p)
-    #(exportable_resexn a3p (bool & int) (EmptyNode Leaf Leaf) #(exportable_pair a3p bool int Leaf Leaf))
+    #(exportable_pair a3p bool int Leaf Leaf)
     _ _
 
+let play_guess_st (a3p:threep) : spec_tree =
+  Node (play_guess_spec a3p) 
+    (EmptyNode
+        (Node (player_spec a3p) Leaf Leaf) Leaf)
+    (EmptyNode Leaf Leaf)
+
+let play_guess_hoc_tree : hoc_tree c3p (play_guess_st c3p) =
+  admit ();
+  Node (| play_guess_spec c3p, play_guess_hoc |)
+    (EmptyNode
+      (Node (| player_spec c3p, player_hoc |) Leaf Leaf) 
+      Leaf)
+    (EmptyNode Leaf Leaf)
+
+let sit2 : src_interface2 = {
+  specs = play_guess_st;
+  hocs = play_guess_hoc_tree;
+  pt = play_guess_type;
+  c_pt = exportable_play_guess;
+}
